template-coq/theories/Typing.v
@@ -703,6 +703,7 @@ Definition check_one_fix d :=
   end.
 
 Definition wf_fixpoint (Σ : global_env) mfix :=
+  forallb (isLambda ∘ dbody) mfix &&
   let checks := map check_one_fix mfix in
   match map_option_out checks with
   | Some (ind :: inds) =>
